theory/x64DecodeProof.thy
@@ -10,12 +10,13 @@ declare if_split_asm [split]
 
 lemma x64_encode_decode_consistency:
   "list_in_list l_bin pc l \<Longrightarrow> Some l_bin = x64_encode ins \<Longrightarrow>  x64_decode pc l = Some (length l_bin, ins)"
-  apply (cases ins; simp_all)
+  apply (cases ins; simp_all add: nth_error_def)
 
   subgoal for dst src
   \<comment> \<open> Pmovl_rr \<close> 
     apply (unfold Let_def)
-    apply (cases "construct_rex_to_u8 False (and (u8_of_ireg src) 8 \<noteq> 0) False (and (u8_of_ireg dst) 8 \<noteq> 0) = 64"; simp_all add: construct_rex_to_u8_def construct_modsib_to_u8_def; erule conjE)
+    apply (cases "construct_rex_to_u8 False (and (u8_of_ireg src) 8 \<noteq> 0) False (and (u8_of_ireg dst) 8 \<noteq> 0) = 64";
+        simp_all add: nth_error_def construct_rex_to_u8_def construct_modsib_to_u8_def; erule conjE)
     subgoal by (cases src; cases dst; auto simp add: x64_decode_def bitfield_insert_u8_def Let_def ireg_of_u8_def)
     subgoal by (cases src; cases dst; auto simp add: x64_decode_def bitfield_insert_u8_def Let_def ireg_of_u8_def)
     done
