theory/x64Disassembler.thy
@@ -12,8 +12,7 @@ value "[(1::nat)]!(1::nat)" returns an error, we should have a nth_error? *)
 
 definition x64_decode :: "nat \<Rightarrow> x64_bin \<Rightarrow> (nat * instruction) option" where
 "x64_decode pc l_bin = (
-  let h = l_bin!pc in
-    \<comment> \<open> R1 [opcode] \<close>
+  case nth_error l_bin pc of None \<Rightarrow> None | Some h \<Rightarrow> \<comment> \<open> R1 [opcode] \<close>
     if h = 0x90 then 
       \<comment> \<open> P2884 `NOP – No Operation` -> `1001 0000` \<close> 
       Some (1, Pnop)
@@ -24,10 +23,10 @@ definition x64_decode :: "nat \<Rightarrow> x64_bin \<Rightarrow> (nat * instruc
       Some (1, Pret)
     \<comment> \<open> R7 legacy \<close>
     else if h = 0x66 then  \<comment> \<open> 16-bit mode \<close>
-      let h1 = l_bin!(pc+1) in
+      case nth_error l_bin (pc+1) of None \<Rightarrow> None | Some h1 \<Rightarrow>
         if unsigned_bitfield_extract_u8 4 4 h1 \<noteq> 0b0100 then  
           \<comment> \<open> R7.1 [legacy + opcode + modrm + imm] \<close>
-          let reg = l_bin!(pc+2) in
+          case nth_error l_bin (pc+2) of None \<Rightarrow> None | Some reg \<Rightarrow>
           let modrm = unsigned_bitfield_extract_u8 6 2 reg in
           let reg1  = unsigned_bitfield_extract_u8 3 3 reg in
           let reg2  = unsigned_bitfield_extract_u8 0 3 reg in
@@ -35,7 +34,7 @@ definition x64_decode :: "nat \<Rightarrow> x64_bin \<Rightarrow> (nat * instruc
           let dst   = bitfield_insert_u8 3 1 reg2 0 in
             if h1 = 0xc1 then 
            \<comment> \<open> P2887 `ROL : register by immediate count` -> `0x66 1100 000w : 11 000 reg : imm8` \<close>
-              let imm = l_bin!(pc+3) in
+              case nth_error l_bin (pc+3) of None \<Rightarrow> None | Some imm \<Rightarrow>
                 if modrm = 0b11 \<and> src = 0b000 then
                   case ireg_of_u8 dst of None \<Rightarrow> None | Some dst \<Rightarrow> (
                     Some (4, Prolw_ri dst imm))
@@ -43,31 +42,32 @@ definition x64_decode :: "nat \<Rightarrow> x64_bin \<Rightarrow> (nat * instruc
           else if h1 = 0x81 then
             if modrm = 0b11 then
               case ireg_of_u8 dst of None \<Rightarrow> None | Some dst \<Rightarrow> (
-                let i1 = l_bin!(pc+3)  in
-                let i2 = l_bin!(pc+4)  in
+                case nth_error l_bin (pc+3) of None \<Rightarrow> None | Some i1 \<Rightarrow> (
+                case nth_error l_bin (pc+4) of None \<Rightarrow> None | Some i2 \<Rightarrow> (
                   case u16_of_u8_list [i1,i2] of None \<Rightarrow> None |
                     Some imm \<Rightarrow> 
                       \<comment> \<open> P2876 `ADD imm16 to reg16` -> ` 0x66 1000 00sw : 11 000 reg : imm16` \<close>
                       if reg1 = 0b000 then
                         Some (5, Paddw_ri dst imm)
-                      else None)
+                      else None) ))
             else None
           \<comment> \<open> R7.2 [legacy + opcode + modrm + displacement] \<close>
             else if h1 = 0x89 then 
               \<comment> \<open> P2882 ` MOV: reg to memory`  ->  `66H 0100 0RXB : 1000 1001 : mod reg r/m `\<close>
                 if modrm = 0b01  then
-                  let (dis::u32) = scast(l_bin!(pc+3)) in  \<comment> \<open> displacement8 \<close>
+                  case nth_error l_bin (pc+3) of None \<Rightarrow> None | Some dis \<Rightarrow> ( \<comment> \<open> displacement8 \<close> 
                     case ireg_of_u8 src of None \<Rightarrow> None | Some src \<Rightarrow> (
                     case ireg_of_u8 dst of None \<Rightarrow> None | Some dst \<Rightarrow> ( 
-                        Some (4, Pmov_mr (Addrmode (Some dst) None dis) src  M16)))
+                        Some (4, Pmov_mr (Addrmode (Some dst) None (scast dis)) src  M16))))
                 else None
             else None
         else  
           let w = unsigned_bitfield_extract_u8 3 1 h1 in
           let r = unsigned_bitfield_extract_u8 2 1 h1 in
           let x = unsigned_bitfield_extract_u8 1 1 h1 in
-          let b = unsigned_bitfield_extract_u8 0 1 h1 in
-            let op = l_bin!(pc+2) in let reg = l_bin!(pc+3) in 
+          let b = unsigned_bitfield_extract_u8 0 1 h1 in (
+            case nth_error l_bin (pc+2) of None \<Rightarrow> None | Some op \<Rightarrow> (
+            case nth_error l_bin (pc+3) of None \<Rightarrow> None | Some reg \<Rightarrow> (
             let modrm = unsigned_bitfield_extract_u8 6 2 reg in
             let reg1  = unsigned_bitfield_extract_u8 3 3 reg in
             let reg2  = unsigned_bitfield_extract_u8 0 3 reg in
@@ -76,39 +76,39 @@ definition x64_decode :: "nat \<Rightarrow> x64_bin \<Rightarrow> (nat * instruc
               \<comment> \<open> R7.3 [legacy + rex + opcode + modrm + imm] \<close>
               if op = 0xc1 then 
               \<comment> \<open> P2887 `ROL : register by immediate count` -> `0x66 1100 000w : 11 000 reg : imm8` \<close>
-                let imm = l_bin!(pc+4) in
+                case nth_error l_bin (pc+4) of None \<Rightarrow> None | Some imm \<Rightarrow> (
                   if modrm = 0b11 \<and> src = 0b000 then
                     case ireg_of_u8 dst of None \<Rightarrow> None | Some dst \<Rightarrow> (
                       if w = 0 \<and> r = 0 \<and> x = 0 then
                         Some (5, Prolw_ri dst imm)
                       else None)
-                  else None
+                  else None )
               else if op = 0x81 then
                 if modrm = 0b11 then
                   case ireg_of_u8 dst of None \<Rightarrow> None | Some dst \<Rightarrow> (
-                    let i1 = l_bin!(pc+4)  in
-                    let i2 = l_bin!(pc+5)  in
+                    case nth_error l_bin (pc+4) of None \<Rightarrow> None | Some i1 \<Rightarrow> (
+                    case nth_error l_bin (pc+5) of None \<Rightarrow> None | Some i2 \<Rightarrow> (
                       case u16_of_u8_list [i1,i2] of None \<Rightarrow> None |
                         Some imm \<Rightarrow> 
                           \<comment> \<open> P2876 `ADD imm16 to reg16` -> ` 0x66 1000 00sw : 11 000 reg : imm16` \<close>
                           if reg1 = 0b000 \<and> w = 0 \<and> r = 0 \<and> x = 0 then
                             Some (6, Paddw_ri dst imm)
-                          else None)
+                          else None) ))
                 else None
               \<comment> \<open> R7.4 [legacy + rex + opcode + modrm + displacement\<close>
               else if op = 0x89 then 
               \<comment> \<open> P2882 ` MOV: reg to memory`  ->  `66H 0100 0RXB : 1000 1001 : mod reg r/m `\<close>
                 if modrm = 0b01  then
-                  let (imm::u32) = scast (l_bin!(pc+4)) in  \<comment> \<open> displacement8 \<close>
+                  case nth_error l_bin (pc+4) of None \<Rightarrow> None | Some dis \<Rightarrow> (  \<comment> \<open> displacement8 \<close>
                       case ireg_of_u8 src of None \<Rightarrow> None | Some src \<Rightarrow> (
                       case ireg_of_u8 dst of None \<Rightarrow> None | Some dst \<Rightarrow> ( 
                         if w = 0 \<and> x = 0 then
-                          Some (5, Pmov_mr (Addrmode (Some dst) None imm) src  M16)
-                        else None))
+                          Some (5, Pmov_mr (Addrmode (Some dst) None (scast dis)) src  M16)
+                        else None )))
                 else None
-              else None
+              else None )))
     else if h = 0x0f then \<comment> \<open> R8 escape \<close>
-      let op = l_bin!(pc+1) in
+      case nth_error l_bin (pc+1) of None \<Rightarrow> None | Some op \<Rightarrow>
         \<comment> \<open> R8.1 [escape + opcode] \<close>         
         if op = 0x31 then 
           Some (2, Prdtsc)
@@ -122,7 +122,7 @@ definition x64_decode :: "nat \<Rightarrow> x64_bin \<Rightarrow> (nat * instruc
         \<comment> \<open> P2919 `MOVcc : resgister2  to resgister1 ` -> `0100 0R0B 0000 1111: 0100 tttn : 11 reg1 reg2` \<close>
         else if unsigned_bitfield_extract_u8 4 4 op = 0b0100 then
           let flag = (unsigned_bitfield_extract_u8 0 4 op) in 
-          let reg = l_bin!(pc+2) in 
+          case nth_error l_bin (pc+2) of None \<Rightarrow> None | Some reg \<Rightarrow>
           let modrm = unsigned_bitfield_extract_u8 6 2 reg in
           let reg1  = unsigned_bitfield_extract_u8 3 3 reg in
           let reg2  = unsigned_bitfield_extract_u8 0 3 reg in
@@ -138,13 +138,13 @@ definition x64_decode :: "nat \<Rightarrow> x64_bin \<Rightarrow> (nat * instruc
         \<comment> \<open> P2880 `JCC: full displacement` -> `0000 1111 : 1000 tttn : full displacement` \<close>
         else if unsigned_bitfield_extract_u8 4 4 op = 0b1000 then
           let flag = (unsigned_bitfield_extract_u8 0 4 op) in
-          let i1 = l_bin!(pc+2)  in
-          let i2 = l_bin!(pc+3)  in
-          let i3 = l_bin!(pc+4)  in
-          let i4 = l_bin!(pc+5)  in
+          case nth_error l_bin (pc+2) of None \<Rightarrow> None | Some i1 \<Rightarrow> (
+          case nth_error l_bin (pc+3) of None \<Rightarrow> None | Some i2 \<Rightarrow> (
+          case nth_error l_bin (pc+4) of None \<Rightarrow> None | Some i3 \<Rightarrow> (
+          case nth_error l_bin (pc+5) of None \<Rightarrow> None | Some i4 \<Rightarrow> (
             case u32_of_u8_list [i1,i2,i3,i4] of None \<Rightarrow> None | Some d \<Rightarrow>(
             case cond_of_u8 flag of None \<Rightarrow> None | Some t \<Rightarrow>(
-              Some(6, Pjcc t d)))
+              Some(6, Pjcc t d))) ))))
         else None
     else if unsigned_bitfield_extract_u8 4 4 h \<noteq> 0b0100 then  \<comment> \<open> h is not rex  \<close>
         \<comment> \<open> R1 [opcode] \<close>
@@ -163,22 +163,22 @@ definition x64_decode :: "nat \<Rightarrow> x64_bin \<Rightarrow> (nat * instruc
         \<comment> \<open> R4 [opcode + displacement] \<close>
         else if h = 0xe8 then   
           \<comment> \<open> P2878 `CALL: direct`   -> `1110 1000 : displacement32` \<close>
-          let i1 = l_bin!(pc+1)  in
-          let i2 = l_bin!(pc+2)  in
-          let i3 = l_bin!(pc+3)  in
-          let i4 = l_bin!(pc+4)  in
+          case nth_error l_bin (pc+1) of None \<Rightarrow> None | Some i1 \<Rightarrow> (
+          case nth_error l_bin (pc+2) of None \<Rightarrow> None | Some i2 \<Rightarrow> (
+          case nth_error l_bin (pc+3) of None \<Rightarrow> None | Some i3 \<Rightarrow> (
+          case nth_error l_bin (pc+4) of None \<Rightarrow> None | Some i4 \<Rightarrow> (
             case u32_of_u8_list [i1,i2,i3,i4] of None \<Rightarrow> None |
-              Some d \<Rightarrow> ( Some (5, Pcall_i (scast d))) 
+              Some d \<Rightarrow> ( Some (5, Pcall_i (scast d))) ))))
         else if h = 0xe9 then
           \<comment> \<open> P2881 `JMP: direct` -> `1110 1001 : displacement32` \<close>
-          let i1 = l_bin!(pc+1)  in
-          let i2 = l_bin!(pc+2)  in
-          let i3 = l_bin!(pc+3)  in
-          let i4 = l_bin!(pc+4)  in
+          case nth_error l_bin (pc+1) of None \<Rightarrow> None | Some i1 \<Rightarrow> (
+          case nth_error l_bin (pc+2) of None \<Rightarrow> None | Some i2 \<Rightarrow> (
+          case nth_error l_bin (pc+3) of None \<Rightarrow> None | Some i3 \<Rightarrow> (
+          case nth_error l_bin (pc+4) of None \<Rightarrow> None | Some i4 \<Rightarrow> (
             case u32_of_u8_list [i1,i2,i3,i4] of None \<Rightarrow> None |
-              Some d \<Rightarrow> ( Some (5, Pjmp (scast d))) 
+              Some d \<Rightarrow> ( Some (5, Pjmp (scast d))) ))))
         else
-          let reg = l_bin!(pc+1) in
+          case nth_error l_bin (pc+1) of None \<Rightarrow> None | Some reg \<Rightarrow>
           let modrm = unsigned_bitfield_extract_u8 6 2 reg in
           let reg1  = unsigned_bitfield_extract_u8 3 3 reg in
           let reg2  = unsigned_bitfield_extract_u8 0 3 reg in
@@ -194,19 +194,19 @@ definition x64_decode :: "nat \<Rightarrow> x64_bin \<Rightarrow> (nat * instruc
               else if modrm = 0b01 then
                 \<comment> \<open> P2882 ` MOV: reg to memory` ->  `0100 WRXB : 1000 1001 : mod reg r/m` \<close>
                 \<comment> \<open> P2882 ` MOV: qwordregister to memory64` ->  `0100 1RXB 1000 1001 : mod qwordreg r/m` \<close>
-                let (dis::u32) = scast (l_bin!(pc+2)) in  \<comment> \<open> displacement8 \<close>
+                case nth_error l_bin (pc+2) of None \<Rightarrow> None | Some dis \<Rightarrow> ( \<comment> \<open> displacement8 \<close>
                   case ireg_of_u8 src of None \<Rightarrow> None | Some src \<Rightarrow> (
                   case ireg_of_u8 dst of None \<Rightarrow> None | Some dst \<Rightarrow> ( 
-                      Some (3, Pmov_mr (Addrmode (Some dst) None dis) src M32)))
+                      Some (3, Pmov_mr (Addrmode (Some dst) None (scast dis)) src M32))))
               else if modrm = 0b10 then 
-                let d1 = l_bin!(pc+2) in
-                let d2 = l_bin!(pc+3) in
-                let d3 = l_bin!(pc+4) in
-                let d4 = l_bin!(pc+5) in
+                case nth_error l_bin (pc+2) of None \<Rightarrow> None | Some d1 \<Rightarrow> (
+                case nth_error l_bin (pc+3) of None \<Rightarrow> None | Some d2 \<Rightarrow> (
+                case nth_error l_bin (pc+4) of None \<Rightarrow> None | Some d3 \<Rightarrow> (
+                case nth_error l_bin (pc+5) of None \<Rightarrow> None | Some d4 \<Rightarrow> (
                   case u32_of_u8_list [d1,d2,d3,d4] of None \<Rightarrow> None | Some dis \<Rightarrow>(
                   case ireg_of_u8 src of None \<Rightarrow> None | Some src \<Rightarrow> (
                   case ireg_of_u8 dst of None \<Rightarrow> None | Some dst \<Rightarrow> (
-                     Some (6, Pmov_mr (Addrmode (Some dst) None dis) src M32))))
+                     Some (6, Pmov_mr (Addrmode (Some dst) None dis) src M32)))) ))))
               else None
             else if h = 0x01 then
             \<comment> \<open> P2876 `ADD register1 to register2` -> `0100 0R0B : 0000 000w : 11 reg1 reg2` \<close>
@@ -238,14 +238,14 @@ definition x64_decode :: "nat \<Rightarrow> x64_bin \<Rightarrow> (nat * instruc
                    Some (2, Pidivl_r dst))
              \<comment> \<open> P2892 `TEST: immediate and register`   -> `  1111 011w : 11 000 reg : imm ` \<close>
               else if modrm = 0b11 \<and> reg1 = 0b000 then
-                let i1 = l_bin!(pc+2)  in
-                let i2 = l_bin!(pc+3)  in
-                let i3 = l_bin!(pc+4)  in
-                let i4 = l_bin!(pc+5)  in
+                case nth_error l_bin (pc+2) of None \<Rightarrow> None | Some i1 \<Rightarrow> (
+                case nth_error l_bin (pc+3) of None \<Rightarrow> None | Some i2 \<Rightarrow> (
+                case nth_error l_bin (pc+4) of None \<Rightarrow> None | Some i3 \<Rightarrow> (
+                case nth_error l_bin (pc+5) of None \<Rightarrow> None | Some i4 \<Rightarrow> (
                   case ireg_of_u8 dst of None \<Rightarrow> None | Some dst \<Rightarrow> (
                       case u32_of_u8_list [i1, i2, i3,i4] of None \<Rightarrow> None |
                         Some imm \<Rightarrow> 
-                            Some (6, Ptestl_ri dst imm))
+                            Some (6, Ptestl_ri dst imm)) ))))
               else None
             \<comment> \<open> P2891 `SUB register1 from register2` -> `0100 WR0B : 0010 100w : 11 reg1 reg2` \<close> 
             else if h = 0x29 then
@@ -312,18 +312,18 @@ definition x64_decode :: "nat \<Rightarrow> x64_bin \<Rightarrow> (nat * instruc
             \<comment> \<open> R3 [opcode + modrm + imm] \<close>
             \<comment> \<open> P2882 `MOV immediate to register` -> ` 1100 011w : 11 000 reg : imm` \<close>
             else if h = 0xc7 then
-              let i1 = l_bin!(pc+2)  in
-              let i2 = l_bin!(pc+3)  in
-              let i3 = l_bin!(pc+4)  in
-              let i4 = l_bin!(pc+5)  in
+              case nth_error l_bin (pc+2) of None \<Rightarrow> None | Some i1 \<Rightarrow> (
+              case nth_error l_bin (pc+3) of None \<Rightarrow> None | Some i2 \<Rightarrow> (
+              case nth_error l_bin (pc+4) of None \<Rightarrow> None | Some i3 \<Rightarrow> (
+              case nth_error l_bin (pc+5) of None \<Rightarrow> None | Some i4 \<Rightarrow> (
               case ireg_of_u8 dst of None \<Rightarrow> None | Some dst \<Rightarrow> (
               case u32_of_u8_list [i1, i2, i3, i4] of None \<Rightarrow> None |
                   Some imm \<Rightarrow> 
                     if modrm = 0b11 \<and> reg1 = 0b000 then
                       Some (6, Pmovl_ri dst imm)
-                    else None)
+                    else None) ))))
             else if h = 0xc1 then
-              let imm = l_bin!(pc+2) in ( 
+              case nth_error l_bin (pc+2) of None \<Rightarrow> None | Some imm \<Rightarrow> ( 
                 \<comment> \<open> P2889 `SHL register by immediate count`      -> `1100 000w : 11 100 reg : imm8 ` \<close>
                 if modrm = 0b11 \<and> reg1 = 0b100 then 
                   case ireg_of_u8 dst of None \<Rightarrow> None | Some dst \<Rightarrow> (
@@ -340,10 +340,10 @@ definition x64_decode :: "nat \<Rightarrow> x64_bin \<Rightarrow> (nat * instruc
             else if h = 0x81 then
               if modrm = 0b11 then
                 case ireg_of_u8 dst of None \<Rightarrow> None | Some dst \<Rightarrow> (
-                  let i1 = l_bin!(pc+2)  in
-                  let i2 = l_bin!(pc+3)  in
-                  let i3 = l_bin!(pc+4)  in
-                  let i4 = l_bin!(pc+5)  in
+                  case nth_error l_bin (pc+2) of None \<Rightarrow> None | Some i1 \<Rightarrow> (
+                  case nth_error l_bin (pc+3) of None \<Rightarrow> None | Some i2 \<Rightarrow> (
+                  case nth_error l_bin (pc+4) of None \<Rightarrow> None | Some i3 \<Rightarrow> (
+                  case nth_error l_bin (pc+5) of None \<Rightarrow> None | Some i4 \<Rightarrow> (
                     case u32_of_u8_list [i1,i2,i3,i4] of None \<Rightarrow> None |
                       Some imm \<Rightarrow> 
                         \<comment> \<open> P2876 `ADD immediate to register` -> ` 1000 00sw : 11 000 reg : immediate data` \<close>
@@ -364,32 +364,32 @@ definition x64_decode :: "nat \<Rightarrow> x64_bin \<Rightarrow> (nat * instruc
                         \<comment> \<open> P2878 `CMP: immediate32 with qwordregister`   -> `0100 100B 1000 0001 : 11 111 qwordreg : imm32` \<close>
                         else if reg1 = 0b111 then
                           Some (6, Pcmpl_ri dst imm)
-                        else None)
+                        else None) ))))
               else None
             \<comment> \<open> R5 [opcode + modrm + displacement] \<close>
             \<comment> \<open> P2882 ` MOV: memory to reg`   ->  `0100 0RXB : 1000 101w : mod reg r/m`\<close>
             else if h = 0x88 then
               if modrm = 0b01  then
-                let (dis::u32) = scast (l_bin!(pc+2)) in  \<comment> \<open> displacement8 \<close>
+                case nth_error l_bin (pc+2) of None \<Rightarrow> None | Some dis \<Rightarrow> ( \<comment> \<open> displacement8 \<close>
                   case ireg_of_u8 src of None \<Rightarrow> None | Some src \<Rightarrow> (
                   case ireg_of_u8 dst of None \<Rightarrow> None | Some dst \<Rightarrow> ( 
-                    Some (3, Pmov_mr (Addrmode (Some dst) None dis) src  M8)))
+                    Some (3, Pmov_mr (Addrmode (Some dst) None (scast dis)) src  M8))) )
               else None
             else if h = 0x8b then 
               if modrm = 0b01 then
-                let (dis::u32) = scast (l_bin!(pc+2)) in  \<comment> \<open> displacement8 \<close>
+                case nth_error l_bin (pc+2) of None \<Rightarrow> None | Some dis \<Rightarrow> ( \<comment> \<open> displacement8 \<close>
                     case ireg_of_u8 src of None \<Rightarrow> None | Some src \<Rightarrow> (
                     case ireg_of_u8 dst of None \<Rightarrow> None | Some dst \<Rightarrow> (
-                      Some (3, Pmov_rm src (Addrmode (Some dst) None dis)  M32)))
+                      Some (3, Pmov_rm src (Addrmode (Some dst) None (scast dis))  M32))) )
               else if modrm = 0b10 then \<comment> \<open> displacement32 \<close>
-                let d1 = l_bin!(pc+2) in
-                let d2 = l_bin!(pc+3) in
-                let d3 = l_bin!(pc+4) in
-                let d4 = l_bin!(pc+5) in
+                case nth_error l_bin (pc+2) of None \<Rightarrow> None | Some d1 \<Rightarrow> (
+                case nth_error l_bin (pc+3) of None \<Rightarrow> None | Some d2 \<Rightarrow> (
+                case nth_error l_bin (pc+4) of None \<Rightarrow> None | Some d3 \<Rightarrow> (
+                case nth_error l_bin (pc+5) of None \<Rightarrow> None | Some d4 \<Rightarrow> (
                   case u32_of_u8_list [d1,d2,d3,d4] of None \<Rightarrow> None | Some dis \<Rightarrow>(
                   case ireg_of_u8 src of None \<Rightarrow> None | Some src \<Rightarrow> (
                   case ireg_of_u8 dst of None \<Rightarrow> None | Some dst \<Rightarrow> (
-                     Some (6, Pmov_rm src (Addrmode (Some dst) None dis) M32))))
+                     Some (6, Pmov_rm src (Addrmode (Some dst) None dis) M32)))) ))))
               else None
             else None
     else if unsigned_bitfield_extract_u8 0 4 h = 0 then   \<comment> \<open> h is rex, the low 4-bit must not 0  \<close> 
@@ -398,8 +398,8 @@ definition x64_decode :: "nat \<Rightarrow> x64_bin \<Rightarrow> (nat * instruc
       let w = unsigned_bitfield_extract_u8 3 1 h in
       let r = unsigned_bitfield_extract_u8 2 1 h in
       let x = unsigned_bitfield_extract_u8 1 1 h in
-      let b = unsigned_bitfield_extract_u8 0 1 h in
-      let op = l_bin!(pc+1) in 
+      let b = unsigned_bitfield_extract_u8 0 1 h in (
+      case nth_error l_bin (pc+1) of None \<Rightarrow> None | Some op \<Rightarrow>
       \<comment> \<open> R6.1 [rex + opcode] \<close>
       if op = 0x99 then
         if w = 1 \<and> r = 0 \<and> x = 0 \<and> b = 0 then
@@ -426,33 +426,33 @@ definition x64_decode :: "nat \<Rightarrow> x64_bin \<Rightarrow> (nat * instruc
       else if unsigned_bitfield_extract_u8 3 5 op = 0b10111 then
         let reg2 = unsigned_bitfield_extract_u8 0 3 op in
         let dst  = bitfield_insert_u8 3 1 reg2 b in
-        let i1 = l_bin!(pc+2)  in
-        let i2 = l_bin!(pc+3)  in
-        let i3 = l_bin!(pc+4)  in
-        let i4 = l_bin!(pc+5)  in
-        let i5 = l_bin!(pc+6)  in
-        let i6 = l_bin!(pc+7)  in
-        let i7 = l_bin!(pc+8)  in
-        let i8 = l_bin!(pc+9)  in
+        case nth_error l_bin (pc+2) of None \<Rightarrow> None | Some i1 \<Rightarrow> (
+        case nth_error l_bin (pc+3) of None \<Rightarrow> None | Some i2 \<Rightarrow> (
+        case nth_error l_bin (pc+4) of None \<Rightarrow> None | Some i3 \<Rightarrow> (
+        case nth_error l_bin (pc+5) of None \<Rightarrow> None | Some i4 \<Rightarrow> (
+        case nth_error l_bin (pc+6) of None \<Rightarrow> None | Some i5 \<Rightarrow> (
+        case nth_error l_bin (pc+7) of None \<Rightarrow> None | Some i6 \<Rightarrow> (
+        case nth_error l_bin (pc+8) of None \<Rightarrow> None | Some i7 \<Rightarrow> (
+        case nth_error l_bin (pc+9) of None \<Rightarrow> None | Some i8 \<Rightarrow> (
         case ireg_of_u8 dst of None \<Rightarrow> None | Some dst \<Rightarrow> (
         case u64_of_u8_list [i1, i2, i3, i4, i5, i6, i7, i8] of None \<Rightarrow> None |
             Some imm \<Rightarrow> 
               if w = 1 \<and> r = 0 \<and> x = 0 then
                 Some (10, Pmovq_ri dst imm)
-          else None)
+          else None) ))))))))
       \<comment> \<open> P2885 `PUSH: imm32`   -> `0100 1000 0110 1000 : imm32 ` \<close>
       else if op = 0x68 then 
-        let i1 = l_bin!(pc+2)  in
-        let i2 = l_bin!(pc+3)  in
-        let i3 = l_bin!(pc+4)  in
-        let i4 = l_bin!(pc+5)  in
+        case nth_error l_bin (pc+2) of None \<Rightarrow> None | Some i1 \<Rightarrow> (
+        case nth_error l_bin (pc+3) of None \<Rightarrow> None | Some i2 \<Rightarrow> (
+        case nth_error l_bin (pc+4) of None \<Rightarrow> None | Some i3 \<Rightarrow> (
+        case nth_error l_bin (pc+5) of None \<Rightarrow> None | Some i4 \<Rightarrow> (
           case u32_of_u8_list [i1, i2, i3, i4] of None \<Rightarrow> None |
             Some imm \<Rightarrow> 
               if w = 1 \<and> r = 0 \<and> x = 0 \<and> b = 0 then
                 Some (6, Ppushl_i imm)
-              else None
+              else None ))))
       else if op = 0x0f then 
-        let op1 = l_bin!(pc+2) in
+        case nth_error l_bin (pc+2) of None \<Rightarrow> None | Some op1 \<Rightarrow>
       \<comment> \<open> R8.4 [rex + escape + opcode] \<close>
       \<comment> \<open> P2877 `BSWAP: register `   -> `0000 1111 : 1100 1 reg` \<close>
       \<comment> \<open> P2877 `BSWAP: qwordregister `   -> `0100 100B 0000 1111 : 1100 1 reg` \<close>
@@ -470,7 +470,7 @@ definition x64_decode :: "nat \<Rightarrow> x64_bin \<Rightarrow> (nat * instruc
       \<comment> \<open> P2919 `MOVcc : qwordregister2 to qwordregister1` -> ` 0100 1R0B 0000 1111: 0100 tttn : 11 qwordreg1 qwordreg2` \<close>
         else if unsigned_bitfield_extract_u8 4 4 op1 = 0b0100 then
           let flag = (unsigned_bitfield_extract_u8 0 4 op1)  in 
-          let reg = l_bin!(pc+3) in
+          case nth_error l_bin (pc+3) of None \<Rightarrow> None | Some reg \<Rightarrow>
           let modrm = unsigned_bitfield_extract_u8 6 2 reg in
           let reg1  = unsigned_bitfield_extract_u8 3 3 reg in
           let reg2  = unsigned_bitfield_extract_u8 0 3 reg in
@@ -487,8 +487,8 @@ definition x64_decode :: "nat \<Rightarrow> x64_bin \<Rightarrow> (nat * instruc
                 else None)))
             else None
         else None
-      else
-        let reg = l_bin!(pc+2) in
+      else (
+        case nth_error l_bin (pc+2) of None \<Rightarrow> None | Some reg \<Rightarrow>
         let modrm = unsigned_bitfield_extract_u8 6 2 reg in
         let reg1  = unsigned_bitfield_extract_u8 3 3 reg in
         let reg2  = unsigned_bitfield_extract_u8 0 3 reg in
@@ -510,42 +510,42 @@ definition x64_decode :: "nat \<Rightarrow> x64_bin \<Rightarrow> (nat * instruc
             else if modrm = 0b01 then
               \<comment> \<open> P2882 ` MOV: reg to memory` ->  `0100 WRXB : 1000 1001 : mod reg r/m` \<close>
               \<comment> \<open> P2882 ` MOV: qwordregister to memory64` ->  `0100 1RXB 1000 1001 : mod qwordreg r/m` \<close>
-              let (dis::u32) = scast (l_bin!(pc+3)) in  \<comment> \<open> displacement8 \<close>
+              case nth_error l_bin (pc+3) of None \<Rightarrow> None | Some dis \<Rightarrow> (  \<comment> \<open> displacement8 \<close>
                 case ireg_of_u8 src of None \<Rightarrow> None | Some src \<Rightarrow> (
                 case ireg_of_u8 dst of None \<Rightarrow> None | Some dst \<Rightarrow> ( 
                   if w = 1 \<and> x = 0 then
-                    Some (4, Pmov_mr (Addrmode (Some dst) None dis) src M64)
+                    Some (4, Pmov_mr (Addrmode (Some dst) None (scast dis)) src M64)
                   else if w = 0 \<and> x = 0 then
-                    Some (4, Pmov_mr (Addrmode (Some dst) None dis) src M32)
-                  else None))
+                    Some (4, Pmov_mr (Addrmode (Some dst) None (scast dis)) src M32)
+                  else None)) )
             else if modrm = 0b10 then
               if reg2 \<noteq> 0b100 then 
-                let d1 = l_bin!(pc+3) in
-                let d2 = l_bin!(pc+4) in
-                let d3 = l_bin!(pc+5) in
-                let d4 = l_bin!(pc+6) in
+                case nth_error l_bin (pc+3) of None \<Rightarrow> None | Some d1 \<Rightarrow> (
+                case nth_error l_bin (pc+4) of None \<Rightarrow> None | Some d2 \<Rightarrow> (
+                case nth_error l_bin (pc+5) of None \<Rightarrow> None | Some d3 \<Rightarrow> (
+                case nth_error l_bin (pc+6) of None \<Rightarrow> None | Some d4 \<Rightarrow> (
                   case u32_of_u8_list [d1,d2,d3,d4] of None \<Rightarrow> None | Some dis \<Rightarrow>(
                     case ireg_of_u8 src of None \<Rightarrow> None | Some src \<Rightarrow> (
                     case ireg_of_u8 dst of None \<Rightarrow> None | Some rb \<Rightarrow> (
-                      Some (7, Pmov_mr (Addrmode (Some rb) None dis) src (if w = 1 then M64 else M32)))))
+                      Some (7, Pmov_mr (Addrmode (Some rb) None dis) src (if w = 1 then M64 else M32))))) ))))
               else 
-                let sib= l_bin!(pc+3) in
+                case nth_error l_bin (pc+3) of None \<Rightarrow> None | Some sib \<Rightarrow> (
                 let rbase  = unsigned_bitfield_extract_u8 0 3 sib in
                 let rindex = unsigned_bitfield_extract_u8 3 3 sib in
                 let scale  = unsigned_bitfield_extract_u8 6 2 sib in
                 let index  = bitfield_insert_u8 3 1 rindex x in
                 let base   = bitfield_insert_u8 3 1 rbase  b in
-                  let d1 = l_bin!(pc+4) in
-                  let d2 = l_bin!(pc+5) in
-                  let d3 = l_bin!(pc+6) in
-                  let d4 = l_bin!(pc+7) in
+                case nth_error l_bin (pc+4) of None \<Rightarrow> None | Some d1 \<Rightarrow> (
+                case nth_error l_bin (pc+5) of None \<Rightarrow> None | Some d2 \<Rightarrow> (
+                case nth_error l_bin (pc+6) of None \<Rightarrow> None | Some d3 \<Rightarrow> (
+                case nth_error l_bin (pc+7) of None \<Rightarrow> None | Some d4 \<Rightarrow> (
                     case u32_of_u8_list [d1,d2,d3,d4] of None \<Rightarrow> None | Some dis \<Rightarrow>(
                       if w = 1 then
                         case ireg_of_u8 src   of None \<Rightarrow> None | Some src \<Rightarrow> (
                         case ireg_of_u8 index of None \<Rightarrow> None | Some ri \<Rightarrow> (
                         case ireg_of_u8 base  of None \<Rightarrow> None | Some rb \<Rightarrow> (
                           Some (8, Pmov_mr (Addrmode (Some rb) (Some (ri, scale)) (scast dis)) src M64))))
-                      else None)
+                      else None) )))) )
             else None
           else if op = 0x87 then
           \<comment> \<open> P2893 `XCHG: register1 with register2 `   -> ` 0100 1R0B 1000 011w : 11 reg1 reg2 ` \<close>
@@ -557,25 +557,25 @@ definition x64_decode :: "nat \<Rightarrow> x64_bin \<Rightarrow> (nat * instruc
                 else None)))
           \<comment> \<open> P2893 `XCHG: memory64 with qwordregister `  -> ` 0100 1RXB 1000 011w : 11 reg1 reg2 ` \<close>
           else if modrm = 0b10 then 
-            if reg2 = 0b100 then                           
-              let sib= l_bin!(pc+3) in
+            if reg2 = 0b100 then
+              case nth_error l_bin (pc+3) of None \<Rightarrow> None | Some sib \<Rightarrow> (
               let rbase  = unsigned_bitfield_extract_u8 0 3 sib in
               let rindex = unsigned_bitfield_extract_u8 3 3 sib in
               let scale  = unsigned_bitfield_extract_u8 6 2 sib in
               let index  = bitfield_insert_u8 3 1 rindex x in
               let base   = bitfield_insert_u8 3 1 rbase  b in
-                let d1 = l_bin!(pc+4) in
-                let d2 = l_bin!(pc+5) in
-                let d3 = l_bin!(pc+6) in
-                let d4 = l_bin!(pc+7) in
+                case nth_error l_bin (pc+4) of None \<Rightarrow> None | Some d1 \<Rightarrow> (
+                case nth_error l_bin (pc+5) of None \<Rightarrow> None | Some d2 \<Rightarrow> (
+                case nth_error l_bin (pc+6) of None \<Rightarrow> None | Some d3 \<Rightarrow> (
+                case nth_error l_bin (pc+7) of None \<Rightarrow> None | Some d4 \<Rightarrow> (
                   case u32_of_u8_list [d1,d2,d3,d4] of None \<Rightarrow> None | Some dis \<Rightarrow>(
                     if w = 1  then
                       case ireg_of_u8 src   of None \<Rightarrow> None | Some src \<Rightarrow> (
                       case ireg_of_u8 index of None \<Rightarrow> None | Some ri \<Rightarrow> (
                       case ireg_of_u8 base  of None \<Rightarrow> None | Some rb \<Rightarrow> (
                         Some (8, Pxchgq_rm src (Addrmode (Some rb) (Some (ri, scale)) (scast dis)) M64))))
-                    else None)
-              else None
+                    else None) ) ))))
+            else None
           else None
           else if op = 0x63 then
           \<comment> \<open> P2883 `MOVXD dwordregister2 to qwordregister1` -> ` 0100 1R0B 0110 0011 : 11 quadreg1 dwordreg2` \<close>
@@ -656,17 +656,17 @@ definition x64_decode :: "nat \<Rightarrow> x64_bin \<Rightarrow> (nat * instruc
             \<comment> \<open> P2892 `TEST: immediate and register`   -> ` 0100 000B 1111 011w : 11 000 reg : imm ` \<close>
             \<comment> \<open> P2892 `TEST: immediate32 and qwordregister `   -> ` 0100 100B 1111 0111 : 11 000 qwordreg : imm32 ` \<close>
             else if modrm = 0b11 \<and> reg1 = 0b000 then
-              let i1 = l_bin!(pc+3)  in
-              let i2 = l_bin!(pc+4)  in
-              let i3 = l_bin!(pc+5)  in
-              let i4 = l_bin!(pc+6)  in
+              case nth_error l_bin (pc+3) of None \<Rightarrow> None | Some i1 \<Rightarrow> (
+              case nth_error l_bin (pc+4) of None \<Rightarrow> None | Some i2 \<Rightarrow> (
+              case nth_error l_bin (pc+5) of None \<Rightarrow> None | Some i3 \<Rightarrow> (
+              case nth_error l_bin (pc+6) of None \<Rightarrow> None | Some i4 \<Rightarrow> (
                 case ireg_of_u8 dst of None \<Rightarrow> None | Some dst \<Rightarrow> (
                 case u32_of_u8_list [i1, i2, i3, i4] of None \<Rightarrow> None | Some imm \<Rightarrow> (
                     if w = 1 \<and> r = 0 \<and> x = 0 then
                       Some (7, Ptestq_ri dst imm)
                     else if w = 0 \<and> r = 0 \<and> x = 0 then
                       Some (7, Ptestl_ri dst imm)
-                    else None))
+                    else None)) ))))
             else None
           else if op = 0x09 then
           \<comment> \<open> P2884 `OR register1 to register2` -> ` 0100 WR0B : 0000 100w : 11 reg1 reg2` \<close>
@@ -767,16 +767,16 @@ definition x64_decode :: "nat \<Rightarrow> x64_bin \<Rightarrow> (nat * instruc
         \<comment> \<open> P2885 `PUSH: memory64`   -> `0100 W00BS : 1111 1111 : mod 110 r/m ` \<close>
           else if modrm = 0b10 then 
             if reg2 = 0b100 then                           
-              let sib= l_bin!(pc+3) in
+              case nth_error l_bin (pc+3) of None \<Rightarrow> None | Some sib \<Rightarrow> (
               let rbase  = unsigned_bitfield_extract_u8 0 3 sib in
               let rindex = unsigned_bitfield_extract_u8 3 3 sib in
               let scale  = unsigned_bitfield_extract_u8 6 2 sib in
               let index  = bitfield_insert_u8 3 1 rindex x in
               let base   = bitfield_insert_u8 3 1 rbase  b in
-                let d1 = l_bin!(pc+4) in
-                let d2 = l_bin!(pc+5) in
-                let d3 = l_bin!(pc+6) in
-                let d4 = l_bin!(pc+7) in
+                case nth_error l_bin (pc+4) of None \<Rightarrow> None | Some d1 \<Rightarrow> (
+                case nth_error l_bin (pc+5) of None \<Rightarrow> None | Some d2 \<Rightarrow> (
+                case nth_error l_bin (pc+6) of None \<Rightarrow> None | Some d3 \<Rightarrow> (
+                case nth_error l_bin (pc+7) of None \<Rightarrow> None | Some d4 \<Rightarrow> (
                   case u32_of_u8_list [d1,d2,d3,d4] of None \<Rightarrow> None | Some dis \<Rightarrow>(
                   if reg1 = 0b110 then
                     if w = 1 \<and> r = 0 then
@@ -784,16 +784,16 @@ definition x64_decode :: "nat \<Rightarrow> x64_bin \<Rightarrow> (nat * instruc
                       case ireg_of_u8 base  of None \<Rightarrow> None | Some rb \<Rightarrow> (
                         Some (8, Ppushq_m (Addrmode (Some rb) (Some (ri, scale)) (scast dis)) M64 )))
                     else None
-                  else None)
-              else None
+                  else None) )))) )
+            else None
           else None
         \<comment> \<open> R6.4 [rex + opcode + modrm + imm] \<close>
         else if op = 0xc7 then
           let n = if modrm = 0b01 then 1 else if modrm = 0b10 then 4 else 0 in
-          let i1 = l_bin!(pc+3+n)  in
-          let i2 = l_bin!(pc+4+n)  in
-          let i3 = l_bin!(pc+5+n)  in
-          let i4 = l_bin!(pc+6+n)  in
+          case nth_error l_bin (pc+3+n) of None \<Rightarrow> None | Some i1 \<Rightarrow> (
+          case nth_error l_bin (pc+4+n) of None \<Rightarrow> None | Some i2 \<Rightarrow> (
+          case nth_error l_bin (pc+5+n) of None \<Rightarrow> None | Some i3 \<Rightarrow> (
+          case nth_error l_bin (pc+6+n) of None \<Rightarrow> None | Some i4 \<Rightarrow> (
             case ireg_of_u8 dst of None \<Rightarrow> None | Some dst \<Rightarrow> (
             case u32_of_u8_list [i1, i2, i3, i4] of None \<Rightarrow> None |
               Some imm \<Rightarrow> 
@@ -807,28 +807,28 @@ definition x64_decode :: "nat \<Rightarrow> x64_bin \<Rightarrow> (nat * instruc
                 \<comment> \<open> P2882 `MOV immediate32 to memory64 (zero extend)` -> ` 0100 10XB 1100 0111 : mod 000 r/m : imm32` \<close>
                 else if modrm = 0b01 then
                   if w = 1 then
-                    let (dis::u32) = scast (l_bin!(pc+3))in
-                    Some (8, Pmov_mi (Addrmode (Some dst) None dis) imm M64)
+                    case nth_error l_bin (pc+3) of None \<Rightarrow> None | Some dis \<Rightarrow> (
+                    Some (8, Pmov_mi (Addrmode (Some dst) None (scast dis)) imm M64) )
                   else None
                 else if modrm = 0b10  then
-                  let d1 = l_bin!(pc+3)  in
-                  let d2 = l_bin!(pc+4)  in
-                  let d3 = l_bin!(pc+5)  in
-                  let d4 = l_bin!(pc+6)  in
+                  case nth_error l_bin (pc+3) of None \<Rightarrow> None | Some d1 \<Rightarrow> (
+                  case nth_error l_bin (pc+4) of None \<Rightarrow> None | Some d2 \<Rightarrow> (
+                  case nth_error l_bin (pc+5) of None \<Rightarrow> None | Some d3 \<Rightarrow> (
+                  case nth_error l_bin (pc+6) of None \<Rightarrow> None | Some d4 \<Rightarrow> (
                     case u32_of_u8_list [d1, d2, d3, d4] of None \<Rightarrow> None |
                       Some dis \<Rightarrow> (
                         if w = 1 then
                           Some (11, Pmov_mi (Addrmode (Some dst) None dis) imm M64)
-                        else None)
+                        else None) ))))
                 else None
-              else None)
+              else None) ))))
         else if op = 0x81 then
           if modrm = 0b11 then
             case ireg_of_u8 dst of None \<Rightarrow> None | Some dst \<Rightarrow> (
-              let i1 = l_bin!(pc+3)  in
-              let i2 = l_bin!(pc+4)  in
-              let i3 = l_bin!(pc+5)  in
-              let i4 = l_bin!(pc+6)  in
+              case nth_error l_bin (pc+3) of None \<Rightarrow> None | Some i1 \<Rightarrow> (
+              case nth_error l_bin (pc+4) of None \<Rightarrow> None | Some i2 \<Rightarrow> (
+              case nth_error l_bin (pc+5) of None \<Rightarrow> None | Some i3 \<Rightarrow> (
+              case nth_error l_bin (pc+6) of None \<Rightarrow> None | Some i4 \<Rightarrow> (
                 case u32_of_u8_list [i1,i2,i3,i4] of None \<Rightarrow> None |
                   Some imm \<Rightarrow> (
                     \<comment> \<open> P2876 `ADD immediate to register` -> `0100 000B : 1000 00sw : 11 000 reg : immediate data` \<close>
@@ -864,36 +864,36 @@ definition x64_decode :: "nat \<Rightarrow> x64_bin \<Rightarrow> (nat * instruc
                       else if w = 0 \<and> r = 0 \<and> x = 0 then
                         Some (7, Pcmpl_ri dst imm)
                       else None
-                    else None))
+                    else None)) ))))
           else if modrm = 0b10 then
             if reg2 = 0b100 then
-              let sib= l_bin!(pc+3) in
+              case nth_error l_bin (pc+3) of None \<Rightarrow> None | Some sib \<Rightarrow> (
               let rbase  = unsigned_bitfield_extract_u8 0 3 sib in
               let rindex = unsigned_bitfield_extract_u8 3 3 sib in
               let scale  = unsigned_bitfield_extract_u8 6 2 sib in
               let index  = bitfield_insert_u8 3 1 rindex x in
               let base   = bitfield_insert_u8 3 1 rbase  b in
-                let d1 = l_bin!(pc+4) in
-                let d2 = l_bin!(pc+5) in
-                let d3 = l_bin!(pc+6) in
-                let d4 = l_bin!(pc+7) in
+                case nth_error l_bin (pc+4) of None \<Rightarrow> None | Some d1 \<Rightarrow> (
+                case nth_error l_bin (pc+5) of None \<Rightarrow> None | Some d2 \<Rightarrow> (
+                case nth_error l_bin (pc+6) of None \<Rightarrow> None | Some d3 \<Rightarrow> (
+                case nth_error l_bin (pc+7) of None \<Rightarrow> None | Some d4 \<Rightarrow> (
                   case u32_of_u8_list [d1,d2,d3,d4] of None \<Rightarrow> None | Some dis \<Rightarrow>(
                   if reg1 = 0b000 then
-                    let i1 = l_bin!(pc+8)  in
-                    let i2 = l_bin!(pc+9)  in
-                    let i3 = l_bin!(pc+10)  in
-                    let i4 = l_bin!(pc+11)  in
+                    case nth_error l_bin (pc+8) of None \<Rightarrow> None | Some i1 \<Rightarrow> (
+                    case nth_error l_bin (pc+9) of None \<Rightarrow> None | Some i2 \<Rightarrow> (
+                    case nth_error l_bin (pc+10) of None \<Rightarrow> None | Some i3 \<Rightarrow> (
+                    case nth_error l_bin (pc+11) of None \<Rightarrow> None | Some i4 \<Rightarrow> (
                     case u32_of_u8_list [i1,i2,i3,i4] of None \<Rightarrow> None | Some imm \<Rightarrow> (
                     if w = 1 \<and> r = 0 then
                       case ireg_of_u8 index of None \<Rightarrow> None | Some ri \<Rightarrow> (
                       case ireg_of_u8 base  of None \<Rightarrow> None | Some rb \<Rightarrow> (
                         Some (12, Paddq_mi (Addrmode (Some rb) (Some (ri, scale)) (scast dis)) imm M64 )))
-                    else None)
-                  else None)
-              else None
+                    else None) ))))
+                  else None) )))) )
+            else None
           else None
         else if op = 0xc1 then
-          let imm = l_bin!(pc+3) in ( 
+          case nth_error l_bin (pc+3) of None \<Rightarrow> None | Some imm \<Rightarrow> (
         \<comment> \<open> P2889 `SHL register by immediate count`      -> ` 0100 000B 1100 000w : 11 100 reg : imm8 ` \<close>
         \<comment> \<open> P2889 `SHL qwordregister by immediate count` -> ` 0100 100B 1100 000w : 11 100 reg : imm8 ` \<close>
             if modrm = 0b11 \<and> reg1 = 0b100 then 
@@ -920,73 +920,73 @@ definition x64_decode :: "nat \<Rightarrow> x64_bin \<Rightarrow> (nat * instruc
         else if op = 0x88 then
           \<comment> \<open> P2882 ` MOV: reg to memory`  ->  `0100 0RXB : 1000 1000 : mod reg r/m `\<close>
           if modrm = 0b01 \<and> x = 0 \<and> w = 0 then
-            let (dis::u32) = scast (l_bin!(pc+3)) in  \<comment> \<open> displacement8 \<close>
+            case nth_error l_bin (pc+3) of None \<Rightarrow> None | Some dis \<Rightarrow> (\<comment> \<open> displacement8 \<close>
               case ireg_of_u8 src of None \<Rightarrow> None | Some src \<Rightarrow> (
               case ireg_of_u8 dst of None \<Rightarrow> None | Some dst \<Rightarrow> ( 
-                Some (4, Pmov_mr (Addrmode (Some dst) None dis) src M8)))
+                Some (4, Pmov_mr (Addrmode (Some dst) None (scast dis)) src M8))) )
           else None
         else if op = 0x8b then    
           if modrm = 0b01 \<and> x = 0 then
           \<comment> \<open> P2882 ` MOV: memory to reg`             ->  `0100 0RXB : 1000 101w : mod reg r/m`\<close>
           \<comment> \<open> P2882 ` MOV: memory64 to qwordregister` ->  `0100 1RXB : 1000 1011 : mod qwordreg r/m`\<close>
-            let (dis::u32) = scast (l_bin!(pc+3)) in  \<comment> \<open> displacement8 \<close>
+            case nth_error l_bin (pc+3) of None \<Rightarrow> None | Some dis \<Rightarrow> (  \<comment> \<open> displacement8 \<close>
               case ireg_of_u8 src of None \<Rightarrow> None | Some src \<Rightarrow> (
               case ireg_of_u8 dst of None \<Rightarrow> None | Some dst \<Rightarrow> ( 
-                Some (4, Pmov_rm src (Addrmode (Some dst) None dis)  (if w = 1 then M64 else M32))))  
+                Some (4, Pmov_rm src (Addrmode (Some dst) None (scast dis))  (if w = 1 then M64 else M32))))  )
           else if modrm = 0b10  then
             if reg2 \<noteq> 0b100 then
-              let d1 = l_bin!(pc+3) in
-              let d2 = l_bin!(pc+4) in
-              let d3 = l_bin!(pc+5) in
-              let d4 = l_bin!(pc+6) in
+              case nth_error l_bin (pc+3) of None \<Rightarrow> None | Some d1 \<Rightarrow> (
+              case nth_error l_bin (pc+4) of None \<Rightarrow> None | Some d2 \<Rightarrow> (
+              case nth_error l_bin (pc+5) of None \<Rightarrow> None | Some d3 \<Rightarrow> (
+              case nth_error l_bin (pc+6) of None \<Rightarrow> None | Some d4 \<Rightarrow> (
               case u32_of_u8_list [d1,d2,d3,d4] of None \<Rightarrow> None | Some dis \<Rightarrow>(
               case ireg_of_u8 src of None \<Rightarrow> None | Some src \<Rightarrow> (
               case ireg_of_u8 dst of None \<Rightarrow> None | Some dst \<Rightarrow> ( 
                 if x = 0 then
                   Some (7, Pmov_rm src (Addrmode (Some dst) None dis) (if w = 1 then M64 else M32))
-                else None)))  
+                else None)))  ))))
             else \<comment> \<open> sib \<close>
-              let sib = l_bin!(pc+3) in
+              case nth_error l_bin (pc+3) of None \<Rightarrow> None | Some sib \<Rightarrow> (
               let rbase  = unsigned_bitfield_extract_u8 0 3 sib in
               let rindex = unsigned_bitfield_extract_u8 3 3 sib in
               let scale  = unsigned_bitfield_extract_u8 6 2 sib in
               let index  = bitfield_insert_u8 3 1 rindex x in
               let base   = bitfield_insert_u8 3 1 rbase  b in
-                let d1 = l_bin!(pc+4) in
-                let d2 = l_bin!(pc+5) in
-                let d3 = l_bin!(pc+6) in
-                let d4 = l_bin!(pc+7) in
+                case nth_error l_bin (pc+4) of None \<Rightarrow> None | Some d1 \<Rightarrow> (
+                case nth_error l_bin (pc+5) of None \<Rightarrow> None | Some d2 \<Rightarrow> (
+                case nth_error l_bin (pc+6) of None \<Rightarrow> None | Some d3 \<Rightarrow> (
+                case nth_error l_bin (pc+7) of None \<Rightarrow> None | Some d4 \<Rightarrow> (
                   case u32_of_u8_list [d1,d2,d3,d4] of None \<Rightarrow> None | Some dis \<Rightarrow>(
                     if w = 1  then
                       case ireg_of_u8 src   of None \<Rightarrow> None | Some src \<Rightarrow> (
                       case ireg_of_u8 index of None \<Rightarrow> None | Some ri \<Rightarrow> (
                       case ireg_of_u8 base  of None \<Rightarrow> None | Some rb \<Rightarrow> (
                         Some (8, Pmov_rm src (Addrmode (Some rb) (Some (ri, scale))  dis) M64))))
-                    else None)
+                    else None) ) ))))
           else None
         \<comment> \<open> P2881 `LEA: Load Effective Address: in qwordregister `  -> `0100 1RXB : 1000 1101 : mod qwordreg r/m` \<close>
         else if op = 0x8d then    
           if modrm = 0b01 then
-            let (dis::u32) = scast (l_bin!(pc+3)) in  \<comment> \<open> displacement8 \<close>
+            case nth_error l_bin (pc+3) of None \<Rightarrow> None | Some dis \<Rightarrow> ( \<comment> \<open> displacement8 \<close>
               case ireg_of_u8 src of None \<Rightarrow> None | Some src \<Rightarrow> (
               case ireg_of_u8 dst of None \<Rightarrow> None | Some dst \<Rightarrow> ( 
                 if w = 1 \<and> x = 0 then
-                  Some (4, Pleaq src (Addrmode (Some dst) None dis))
-                else None))  
+                  Some (4, Pleaq src (Addrmode (Some dst) None (scast dis)))
+                else None))  )
           else if modrm = 0b10  then
-            let d1 = l_bin!(pc+3)  in
-            let d2 = l_bin!(pc+4)  in
-            let d3 = l_bin!(pc+5)  in
-            let d4 = l_bin!(pc+6)  in
+            case nth_error l_bin (pc+3) of None \<Rightarrow> None | Some d1 \<Rightarrow> (
+            case nth_error l_bin (pc+4) of None \<Rightarrow> None | Some d2 \<Rightarrow> (
+            case nth_error l_bin (pc+5) of None \<Rightarrow> None | Some d3 \<Rightarrow> (
+            case nth_error l_bin (pc+6) of None \<Rightarrow> None | Some d4 \<Rightarrow> (
               case u32_of_u8_list [d1, d2, d3, d4] of None \<Rightarrow> None | Some dis \<Rightarrow> (
               case ireg_of_u8 src of None \<Rightarrow> None | Some src \<Rightarrow> (
               case ireg_of_u8 dst of None \<Rightarrow> None | Some dst \<Rightarrow> ( 
                 if w = 1 \<and> x = 0 then
                   Some (7, Pleaq src (Addrmode (Some dst) None dis))
-                else None)))
+                else None))) ))))
           else None
     \<comment> \<open> R6.6 [rex + opcode + modrm + displacement + imm] \<close>
-        else None 
+        else None ))
 )"
 
 (*
